The evaluation of linear code terminates with an ip pointer out of the code

typed-assembly/Compiler/CFGNoLoop.v
@@ -1,10 +1,9 @@
 (** Control flow graphs without loops. *)
-Require Import ZArith.
 Require Import List.
+Require Import Compiler.Linear.
 
 Set Implicit Arguments.
 Import ListNotations.
-Local Open Scope Z_scope.
 
 Module CFG.
   Inductive t (S : Set) : (S -> Type) -> (S -> Type) -> Type :=
@@ -18,30 +17,38 @@ Module CFG.
     t Lin_true Lmerge -> t Lin_false Lmerge -> t Lmerge Lout ->
     t Lin Lout.
   
-  Fixpoint eval (S : Set) Lin Lout (p : t Lin Lout)
-    (s : S) (l : Lin s) {struct p} : {s' : S & Lout s'}.
-    destruct p as
+  Fixpoint eval (S : Set) Lin Lout (g : t Lin Lout)
+    (s : S) (l : Lin s) {struct g} : {s' : S & Lout s'}.
+    destruct g as
       [ L
-      | Lin L Lout f p
-      | Lin Lin_true Lin_false Lmerge Lout f p_true p_false p].
+      | Lin L Lout f g
+      | Lin Lin_true Lin_false Lmerge Lout f g_true g_false g].
     - exact (existT _ _ l).
     
     - exact (
         let (_, fl) := f s in
-        eval _ _ _ p _ (fl l)).
+        eval _ _ _ g _ (fl l)).
     
     - exact (
         match f s with
         | inl fl_true =>
-          let (s, l) := eval _ _ _ p_true _ (fl_true l) in
-          eval _ _ _ p _ l
+          let (s, l) := eval _ _ _ g_true _ (fl_true l) in
+          eval _ _ _ g _ l
         | inr fl_false =>
-          let (s, l) := eval _ _ _ p_false _ (fl_false l) in
-          eval _ _ _ p _ l
+          let (s, l) := eval _ _ _ g_false _ (fl_false l) in
+          eval _ _ _ g _ l
         end).
   Defined.
   
+  Fixpoint length (S : Set) (Lin Lout : S -> Type) (g : t Lin Lout) : nat :=
+    match g with
+    | nop _ => 0
+    | op _ _ g => 1 + (length g)
+    | jcc _ _ g_true g_false g => length g_true + length g_false + length g
+    end.
+  
   Module Test.
+    Require Import Arith.Plus.
     Require Import Arith.Compare_dec.
     Local Open Scope nat_scope.
     
@@ -51,11 +58,64 @@ Module CFG.
     Definition g1 : CFG.t L1 L2.
       refine (
         op _ (fun s => existT _ (s + 2) (fun l => _))
-        (@nop _ _)); abstract (
-      unfold L1, L2 in *;
-      omega).
+        (@nop _ _)).
+      unfold L1, L2 in *.
+      replace 5 with (3 + 2); trivial.
+      now apply plus_le_compat_r.
     Defined.
     
     Check eq_refl : 6 = projT1 (eval g1 4 (leb_complete 3 4 eq_refl)).
   End Test.
 End CFG.
+
+Module Compile.
+  Require Import Arith.Wf_nat.
+  Import CFG.
+  
+  Fixpoint Laux (S : Set) (Lin Lout : S -> Type) (g : CFG.t Lin Lout)
+    (ip : nat) : (S -> Type) + nat :=
+    match g with
+    | nop _ => inr ip
+    | op _ _ g =>
+      match ip with
+      | O => inl Lin
+      | Datatypes.S ip => Laux g ip
+      end
+    | jcc _ _ g_true g_false  g =>
+      match ip with
+      | O => inl Lin
+      | Datatypes.S ip =>
+        match Laux g_true ip with
+        | inl L => inl L
+        | inr ip =>
+          match Laux g_false ip with
+          | inl L => inl L
+          | inr ip => Laux g ip
+          end
+        end
+      end
+    end.
+  
+  Definition L (S : Set) (Lin Lout : S -> Type) (g : CFG.t Lin Lout)
+    (ip : nat) : S -> Type :=
+    match Laux g ip with
+    | inl L => L
+    | inr _ => Lout
+    end.
+  
+  Definition lt (S : Set) (L : nat -> S -> Type) : Instr.lt_type L :=
+    fun x y =>
+    projT1 x < projT1 y.
+  
+  Lemma lt_wf (S : Set) (L : nat -> S -> Type) : well_founded (lt L).
+    apply well_founded_ltof.
+  Defined.
+  
+  (*Fixpoint compile (S : Set) (Lin Lout : S -> Type) (g : CFG.t Lin Lout)
+    : Program.t (lt (L g)) 0.*)
+End Compile.
+
+
+
+
+
